ok
git-svn-id: svn://scm.gforge.inria.fr/svn/cfml@271 ba02c806-7d2b-4818-9a48-35b22e6bdc79

imper/Counter_proof.v
@@ -43,428 +43,65 @@ Qed.
 (* ** List iterator *)
 
 Lemma iter_spec : forall A,
-  Spec iter (f:func) (l:list A) | R>>
+  Spec iter (f:func) (l0:list A) | R>>
     forall H (Q:unit->hprop),
     (forall (S:list A -> _ -> _ -> Prop),
        is_local_1 S ->
-       (forall H Q, H ==> Q tt -> S nil H Q) ->
-       (forall H Q x l,
-          (localize H Q (fun (H:hprop) (Q:unit->hprop) => 
-             exists Q':unit->hprop,
-             app_1 f x H Q' /\ S l (Q' tt) Q) -> S (x::l) H Q)) ->
-      S l H Q) -> 
-   R H Q.
+       (forall l H' Q',
+          match l with
+          | nil => (Ret tt) H' Q'
+          | x::l' => ((App f x;) ;; S l') H' Q'
+          end -> S l H' Q') ->
+       S l0 H Q) ->
+    R H Q.
 Proof.
-  intros. xintros. intros f l H Q M.
-(*
-  specializes M (@app_2 Func (list A) unit iter f).  
-  forwards J: (iter_cf (K:= fun f' l' R => f' = f -> l' = l -> R H Q));
-   [ | | ]. skip. skip. lets: (spec_elim_2 J).
-*)
- sets_eq S: (app_2 (A1:=val) (A2:=list A) (B:=unit) iter f). 
- (*   specializes M S. *)
-  (* gen M. induction_wf IH: (@list_sub_wf A) l. intros M. apply M. *)
-  apply M; clear M H Q.
-  rewrite EQS. intros. xlocal.
-  intros H Q v.
-    rewrite EQS. eapply app_spec_2. xcf. intros. subst.
-    xmatch. xret~.
-  intros H Q x t J.
-    rewrite EQS. eapply app_spec_2. xcf. intros. subst.
-   xmatch.
-   applys local_weaken_formula J. clears H Q. intros H Q. intros (Q'&J1&J2). 
-   exists (Q' tt). split. skip. (* todo : fix apply J1. *) apply J2.
+  intros. xintros. intros f l0. introv M.
+  sets_eq S: (app_2 (A1:=func) (A2:=list A) (B:=unit) iter f).
+  apply M; clear M H Q. rewrite EQS. intros_all. xlocal.
+  intros l H' Q' HS. rewrite EQS. eapply app_spec_2.
+  xcf. intros. subst. xmatch; auto.
 Qed.
 
 Hint Extern 1 (RegisterSpec iter) => Provide iter_spec.
 
 
+(********************************************************************)
+(* ** Ignore function *)
+
+Lemma ignore_spec : forall a,
+  Specs ignore (x:a) >> [] (#[]).
+Proof. intros. xcf. intros. xret~. Qed.
+
+Hint Extern 1 (RegisterSpec ignore) => Provide ignore_spec.
 
 
-Definition counter_spec I f :=
-  Spec f () |R>> forall n, R (I n) (\=n \*+ (I (n+1))).
+(********************************************************************)
+(* ** Iterating calls to counter functions *)
 
-Definition Counter (n:int) (f:func) :=
-  Hexists I:int->hprop, (I n) \* [counter_spec I f].
-
-Lemma gensym_spec : Spec gensym () |R>>
-  R [] (fun f => f ~> Counter 0).
-Proof.
-  unfold Counter, hdata. xgo.
-  sets I: (fun n:int => x ~> Ref Id n).
-  xfun (counter_spec I). xgo*. xret. hsimpl~ I.
-Qed.
-
-Definition localize B (H:hprop) (Q:B->hprop) (R:~~B) :=
-  local R H Q.
-
-Lemma local_weaken_formula : forall B (F1 F2:~~B) H Q,
-  local F1 H Q -> (F1 ===> F2) -> local F2 H Q.
-Proof.
-  introv M W. introv Hh.
-  destruct (M h Hh) as (?&?&?&?&?&?&?).
-  exists___. splits; [ | apply W; apply H1 |]. eauto. eauto. 
-Qed.
-
-Lemma app_spec_2' : forall A1 A2 B f (v1:A1) (v2:A2) (H:hprop) (Q : B->hprop),
-  spec_2 (fun x1 x2 R => x1 = v1 -> x2 = v2 -> 
-    (forall H Q, R H Q -> app_2 f v1 v2 H Q) -> R H Q) f ->
-  app_2 f v1 v2 H Q.
-Proof. introv S. forwards~ K : (spec_elim_2 S). Qed.
-(* to simpler *)
-
-
-Lemma iter_spec' : forall A,
-  Spec iter (f:func) (l:list A) | R>>
-    forall H (Q:unit->hprop),
-    (forall (S:list A -> _ -> _ -> Prop),
-       (forall l, is_local (S l)) ->
-       (match l with 
-       | nil => H ==> Q tt
-       | x::l' =>      
-          localize H Q (fun (H:hprop) (Q:unit->hprop) => 
-             exists Q':unit->hprop,
-             app_1 f x H Q' /\ S l (Q' tt) Q)
-       end -> S l H Q) -> 
-      S l H Q) -> 
-   R H Q.
-Proof.
-Admitted.
-(*
-  intros. xintros. intros f l H Q M.
-(*
-  specializes M (@app_2 Func (list A) unit iter f).  
-  forwards J: (iter_cf (K:= fun f' l' R => f' = f -> l' = l -> R H Q));
-   [ | | ]. skip. skip. lets: (spec_elim_2 J).
-*)
- sets_eq S: (app_2 (A1:=val) (A2:=list A) (B:=unit) iter f). 
- (*   specializes M S. *)
-  (* gen M. induction_wf IH: (@list_sub_wf A) l. intros M. apply M. *)
-  apply M; clear M.
-  intros v.
-    rewrite EQS. eapply app_spec_2. xcf. intros. subst.
-    xmatch. xret~.
-  intros x t J.
-    rewrite EQS. eapply app_spec_2. xcf. intros. subst.
-   xmatch.
-   applys local_weaken_formula J. clears H Q. intros H Q. intros (Q'&J1&J2). 
-   exists (Q' tt). split. skip. (* todo : fix apply J1. *) apply J2.
-Qed.
-*)
-
-
-
-Lemma iter_spec : forall A,
-  Spec iter (f:func) (l:list A) | R>>
-    forall H (Q:unit->hprop),
-    (forall (S:list A -> _ -> _ -> Prop),
-       (forall l, is_local (S l)) ->
-       (forall H Q, H ==> Q tt -> S nil H Q) ->
-       (forall H Q x l,
-          (localize H Q (fun (H:hprop) (Q:unit->hprop) => 
-             exists Q':unit->hprop,
-             app_1 f x H Q' /\ S l (Q' tt) Q) -> S (x::l) H Q)) ->
-      S l H Q) -> 
-   R H Q.
-Proof.
-  intros. xintros. intros f l H Q M.
-(*
-  specializes M (@app_2 Func (list A) unit iter f).  
-  forwards J: (iter_cf (K:= fun f' l' R => f' = f -> l' = l -> R H Q));
-   [ | | ]. skip. skip. lets: (spec_elim_2 J).
-*)
- sets_eq S: (app_2 (A1:=val) (A2:=list A) (B:=unit) iter f). 
- (*   specializes M S. *)
-  (* gen M. induction_wf IH: (@list_sub_wf A) l. intros M. apply M. *)
-  apply M; clear M H Q.
-  rewrite EQS. intros. xlocal.
-  intros H Q v.
-    rewrite EQS. eapply app_spec_2. xcf. intros. subst.
-    xmatch. xret~.
-  intros H Q x t J.
-    rewrite EQS. eapply app_spec_2. xcf. intros. subst.
-   xmatch.
-   applys local_weaken_formula J. clears H Q. intros H Q. intros (Q'&J1&J2). 
-   exists (Q' tt). split. skip. (* todo : fix apply J1. *) apply J2.
-Qed.
-
-Hint Extern 1 (RegisterSpec iter) => Provide iter_spec.
-
-
-Lemma hsimpl_to_qunit' : forall (H:hprop),
-  H ==> (fun _ => H) tt.
-Proof. intros. subst. auto. Qed.
-Hint Resolve hsimpl_to_qunit'.
-
-Lemma test_spec : 
-  Spec test (l:list func) |R>>
-    forall L, 
+Lemma step_all_spec : 
+  Spec step_all (l:list func) |R>> forall L, 
     R (l ~> List Counter L) (# l ~> List Counter (LibList.map (fun i => i+1) L)).
 Proof.
-  xcf. intros l L. 
-  xfun (fun g => Spec g f |R>> 
-     forall (Q':int->hprop) H (Q:unit->hprop),
-     app_1 f tt H Q' -> 
-     (forall x, Q' x ==> Q tt) ->
-     R H Q).
-     intros M W. xlet. apply M. xret~.
-   renames _f0 to g, S_f0 to Sg.
-  xuntag. apply ( spec_elim_2 (@iter_spec func)).
-  intros S LS Jn Jc.
-  gen L. induction l as [|f l]; intros L.
-  apply Jn. clear Jn Jc.
-   hchange (@unfocus_nil' _ L _ Counter).
-   hextract. subst. Opaque List.
-   hchange (@focus_nil _ _ Counter). hsimpl.
- apply Jc. clear Jn Jc.
-  unfold localize.  
-  xchange (focus_cons' f l).
-   xextract as n L' E. subst L.
-   unfold Counter at 1.
-   unfold hdata at 1.
-   xextract as I HI. unfolds in HI.
-   apply local_erase. esplit. split.
-   eapply (spec_elim_1 Sg).
-change (app_1 (B:=Z) f tt)
- with (tag tag_apply None (app_1 (B:=Z) f tt)).
-xapp.
-intros x. simpl. hextract. apply~ hsimpl_to_qunit.
- simpl. eapply local_wframe.
-auto. apply ( IHl L'). hsimpl.
- hsimpl.
+  xcf. intros. 
+  xfun (fun g => Spec g f |R>> forall (Q':int->hprop) H (Q:unit->hprop),
+     (App f tt;) H Q' -> (forall x, Q' x ==> Q tt) -> R H Q).
+     intros M W. xlet. apply M. xapp. hsimpl.
+      applys pred_le_trans (W _x3). hsimpl.
+     renames _f0 to g, S_f0 to Sg.
+  apply (spec_elim_2 (@iter_spec func)). intros S LS HS.
+  gen l. induction_wf: (@list_sub_wf int) L. intros.
+  apply HS. clear HS. destruct l.
+  (* case nil *)
+  xret. hchange (@unfocus_nil' _ L _ Counter). hextract. subst.
+  hchange (@focus_nil _ _ Counter). hsimpl.
+  (* case cons *)
+  xchange (focus_cons' f l) as n L' E. 
+  xseq (# f ~> Counter (n + 1) \* l ~> List Counter L'). 
+  eapply (spec_elim_1 Sg).
+  xframe (l ~> List Counter L'). apply Counter_apply. xok. intros. xsimpl.
+  subst L. xapply_local~ (>>> IH L'). hsimpl.
+  intros _. rew_map. hchange (unfocus_cons f l (n+1)). hsimpl.
 Qed.
 
 
 
- xuntag. 
-
- let f := spec_goal_fun tt in
-      xfind f; let H := fresh in intro H.
-Ieapply spec_elim_1.      
-xapp_spec_core H idcont.
-; clear H
-
-xapp_core __ idcont.  
-xapp_manual.
-
-    apply (spec_elim_1 HI).
- (* todo: add tags*)
-  apply (spec_elim_1 Sg).
-  xchange (focus_cons' f l). 
-
- (* todo*)
-
-  xextract I.
- 
-  
-
-
- hsimpl.  destruct  appl.
- apply H.
-  apply local_erase. n a pply spec_elim
-  xapp_manual.
-  apply KR; clear KR. intros S Jn Jc. 
-  
-  destruct l.
-  
-
-Qed.
-
-(*
-  (* gen M. induction_wf IH: (@list_sub_wf A) l. intros M. apply M. *)
-  apply M.
-  intros v.
-    rewrite EQS. eapply app_spec_2. xcf. intros. subst.
-    xmatch. xret~.
-  intros x t J.
-     rewrite EQS. eapply app_spec_2. xcf. intros. subst.
-     xmatch.
-    eapply local_weaken_formula. apply J. clears H Q. intros H Q.
-    intros (Q'&J1&J2). 
-    exists (Q' tt). split. skip. (* todo : fix apply J1. *) apply J2.
-Qed
-     rewrite EQS. eapply app_spec_2. xcf. intros. subst.
-     xmatch.
-    eapply local_weaken_formula. apply J. clears H Q. intros H Q.
-    intros (Q'&J1&J2). 
-    exists (Q' tt). split. skip. (* todo : fix apply J1. *) apply J2.
-Qed.*)
-
-  rewrite 
-
-QeEQS.
-  forwards J: iter_cf. skip. skip.
-  
-eapply (spec_elim_2 J).
- eapply app_spec_2.
-  apply 
-  xcf. intros. subst. 
-  xmatch. xret. auto.
-subst. xmatch. xret~.  
-  forwards J: (iter_cf (K:= fun f' l' R => f' = f -> l' = l -> R H Q));
-   [ | | apply~ (spec_elim_2 J) ].
-  intros_all~.
-
-; [ | | lets: (sp_elim_2 J) ].
-skip.
-skip.
-.
-
-eapply app_spec_2. 
-apply spec_intro_2. skip. skip. intros.
-apply H0.
- skip.
-  sets_eq S: (app_2 (A1:=val) (A2:=list A) (B:=unit) iter f). 
- (*   specializes M S. *)
-  (* gen M. induction_wf IH: (@list_sub_wf A) l. intros M. apply M. *)
-  apply M.
-  intros v.
-    rewrite EQS. eapply app_spec_2. xcf. intros. subst.
-    xmatch. xret~.
-  intros x t J.
-    rewrite EQS. eapply app_spec_2. xcf. intros. subst.
-   xmatch.
-   applys local_weaken_formula J. clears H Q. intros H Q. intros (Q'&J1&J2). 
-   exists (Q' tt). split. skip. (* todo : fix apply J1. *) apply J2.
-Qed.
-
-Lemma test_spec : 
-  Spec test (l:list func) |R>>
-    forall L, 
-    R (l ~> List Counter L) (l ~> List Counter (map S L)).
-
-
-(*
-  (* gen M. induction_wf IH: (@list_sub_wf A) l. intros M. apply M. *)
-  apply M.
-  intros v.
-    rewrite EQS. eapply app_spec_2. xcf. intros. subst.
-    xmatch. xret~.
-  intros x t J.
-     rewrite EQS. eapply app_spec_2. xcf. intros. subst.
-     xmatch.
-    eapply local_weaken_formula. apply J. clears H Q. intros H Q.
-    intros (Q'&J1&J2). 
-    exists (Q' tt). split. skip. (* todo : fix apply J1. *) apply J2.
-Qed.*)
-
-  rewrite EQS.
-  forwards J: iter_cf. skip. skip.
-  
-eapply (spec_elim_2 J).
- eapply app_spec_2.
-  apply 
-  xcf. intros. subst. 
-  xmatch. xret. auto.
-subst. xmatch. xret~.
-
- apply M.
- 
- induction l; intros.
-  apply M.
-  intros V. rewrite EQS. eapply app_spec_2. xcf. intros. subst. xmatch. xret~.
-
-  intros x l V. rewrite EQS. eapply app_spec_2. xcf. intros. subst. xmatch.  
-  eapply local_weaken_formula. apply V. clears H Q. intros H Q.
-  intros (Q'&J1&J2). 
-  exists (Q' tt). split. skip. (* todo : fix apply J1. *)
-  apply J2.
-
-  
-  eapply M.
-  Qed.
-  
-
-
-
-
-(* Details of the proof:
-
-  xcf. xgo. 
-  xfun (counter_spec (fun n => x ~> RefOn n)).
-    xapp. intro_subst. xapp. xret. ximpl~.
-  xret. ximpl~.
-
-*)
-
-(* details of hsimpl:
-
-hsimpl_setup tt.
-hsimpl_step tt.
-apply hsimpl_cancel_eq_1.
-eapply refl_equal.
-hsimpl_step tt.
-hsimpl_step tt.
-hsimpl_step tt.
-
-*)
-
-
-
-Lemma iter_spec : forall A,
-  Spec iter (f:func) (l:list A) | R>>
-    forall H (Q:unit->hprop),
-    (forall (S:list A -> _ -> _ -> Prop),
-       (forall H Q, H ==> Q tt -> S nil H Q) ->
-       (forall H Q x l,
-          (localize H Q (fun (H:hprop) (Q:unit->hprop) => 
-             exists Q':unit->hprop,
-             app_1 f x H Q' /\ S l (Q' tt) Q) -> S (x::l) H Q)) ->
-      S l H Q) -> 
-   R H Q.
-Proof.
-  intros. xintros. intros f l H Q M.
-(*
-  specializes M (@app_2 Func (list A) unit iter f).  
-  forwards J: (iter_cf (K:= fun f' l' R => f' = f -> l' = l -> R H Q));
-   [ | | ]. skip. skip. lets: (spec_elim_2 J).
-*)
- sets_eq S: (app_2 (A1:=val) (A2:=list A) (B:=unit) iter f). 
- (*   specializes M S. *)
-  (* gen M. induction_wf IH: (@list_sub_wf A) l. intros M. apply M. *)
-  apply M; clear M H Q.
-  intros H Q v.
-    rewrite EQS. eapply app_spec_2. xcf. intros. subst.
-    xmatch. xret~.
-  intros H Q x t J.
-    rewrite EQS. eapply app_spec_2. xcf. intros. subst.
-   xmatch.
-   applys local_weaken_formula J. clears H Q. intros H Q. intros (Q'&J1&J2). 
-   exists (Q' tt). split. skip. (* todo : fix apply J1. *) apply J2.
-Qed.
-
-
-
-Lemma iter_spec : forall A,
-  Spec iter (f:func) (l:list A) | R>>
-    forall H (Q:unit->hprop),
-    (forall (S:list A -> _ -> _ -> Prop),
-       (forall, H ==> Q tt -> S nil H Q) ->
-       (forall x l,
-          (localize H Q (fun (H:hprop) (Q:unit->hprop) => 
-             exists Q':unit->hprop,
-             app_1 f x H Q' /\ S l (Q' tt) Q) -> S (x::l) H Q)) ->
-      S l H Q) -> 
-   R H Q.
-Proof.
-  intros. xintros. intros f l H Q M.
-(*
-  specializes M (@app_2 Func (list A) unit iter f).  
-  forwards J: (iter_cf (K:= fun f' l' R => f' = f -> l' = l -> R H Q));
-   [ | | ]. skip. skip. lets: (spec_elim_2 J).
-*)
- sets_eq S: (app_2 (A1:=val) (A2:=list A) (B:=unit) iter f). 
- (*   specializes M S. *)
-  (* gen M. induction_wf IH: (@list_sub_wf A) l. intros M. apply M. *)
-  apply M; clear M.
-  intros v.
-    rewrite EQS. eapply app_spec_2. xcf. intros. subst.
-    xmatch. xret~.
-  intros x t J.
-    rewrite EQS. eapply app_spec_2. xcf. intros. subst.
-   xmatch.
-   applys local_weaken_formula J. clears H Q. intros H Q. intros (Q'&J1&J2). 
-   exists (Q' tt). split. skip. (* todo : fix apply J1. *) apply J2.
-Qed.
-
-Hint Extern 1 (RegisterSpec iter) => Provide iter_spec.
